proof/theories/Syntax.v
@@ -164,8 +164,9 @@ Inductive matchcond : Type :=
 Inductive vsrc : Type :=
 | VImm   (v : data)
 | VField (f : field) (ts : list transform)
-| VMap   (f : field) (name : string) (entries : list (data * data)).
-                            (* value looked up by [field] in a named map *)
+| VMap   (fields : list field) (name : string) (entries : list (data * data)).
+                            (* value looked up by the concatenation of [fields] in
+                               a named map *)
 
 Inductive stmt : Type :=
 | SCounter (pkts bytes : nat)
